Progress towards ReliableBroadcast
I'm commiting now, despite this not being finished, because I
intend to make some changes in the typeclass hierarchy, to more
elegantly represent Byzantine adversaries.

Examples/ReliableBroadcast.lean
@@ -4,6 +4,7 @@ import LeanSts.Tactic
 import LeanSts.BFT.Network
 
 -- https://github.com/verse-lab/verify-ABC-in-Coq/blob/main/Protocols/RB/Protocol.v
+-- https://decentralizedthoughts.github.io/2020-09-19-living-with-asynchrony-brachas-reliable-broadcast/
 
 section ReliableBroadcast
 variable {Address Round Value : Type}
@@ -13,59 +14,90 @@ def InternalTransition := Round
 
 inductive Message
   | InitialMsg (r : Round) (v : Value)
-  | EchoMsg (orig : Address) (r : Round) (v : Value)
-  | VoteMsg (orig : Address) (r : Round) (v : Value)
+  /-- The `originator` is the leader, i.e. the party that initiates the broadcast.
+    It is NOT the sender of the message. -/
+  | EchoMsg (originator : Address) (r : Round) (v : Value)
+  /-- The `originator` is the leader, i.e. the party that initiates the broadcast.
+    It is NOT the sender of the message. -/
+  | VoteMsg (originator : Address) (r : Round) (v : Value)
 deriving DecidableEq
 
 structure NodeState :=
+  /-- This node's address -/
   id : Address
+  /-- The set of all nodes -/
+  allNodes : List Address
+
   sent : Round → Bool
   echoed : (Address × Round) → Option Value
   voted : (Address × Round) → Option Value
-  msgCount : @Message Address Round Value → List Address
+  msgReceivedFrom : (@Message Address Round Value) → List Address
   output : (Address × Round) → List Value
 
-def init (id : Address) : @NodeState Address Round Value := {
+def RBNetworkState := @AsynchronousNetwork.World Address (Packet Address (@Message Address Round Value)) (@NodeState Address Round Value)
+instance RBAdversary : @ByzantineAdversary Address (@Message Address Round Value) (@NetworkState Address (Packet Address (@Message Address Round Value)) (@NodeState Address Round Value)) :=
+  sorry
+
+def init (id : Address) (nodes : List Address) : @NodeState Address Round Value := {
   id := id
+  allNodes := nodes
   sent := λ _ => false
   echoed := λ _ => none
   voted := λ _ => none
-  msgCount := λ _ => []
+  msgReceivedFrom := λ _ => []
   output := λ _ => []
 }
 
-def procInt (st : @NodeState Address Round Value) (r : @InternalTransition Round) :
-  (@NodeState Address Round Value) × List (Packet Address (@Message Address Round Value)) := sorry
+def procInt (inputValue : Address → Value) (st : @NodeState Address Round Value) (r : @InternalTransition Round) :
+  (@NodeState Address Round Value) × List (Packet Address (@Message Address Round Value)) :=
+  if st.sent r then
+    (st, [])
+  else
+    let st' := { st with sent := st.sent[r ↦ true] };
+    let msg := Message.InitialMsg r (inputValue st.id);
+    let pkts := Packet.broadcast st.id st.allNodes msg
+    (st', pkts)
+
+/-- Internal message handler for Reliable Broadcast. Returns `none` if nothing to do. -/
+def handleMessage (st : @NodeState Address Round Value) (src : Address) (msg : @Message Address Round Value) :
+  Option ((@NodeState Address Round Value) × List (Packet Address (@Message Address Round Value))) :=
+  match msg with
+  | Message.InitialMsg r v =>
+    if let .none := st.echoed (src, r) then
+      let st' := {st with echoed := st.echoed[(src, r) ↦ some v]};
+      let msg := Message.EchoMsg st.id r v;
+      let pkts := Packet.broadcast st.id st.allNodes msg
+      (st', pkts)
+    else none
+  /- We keep track of how many times we've seen  -/
+  | _ =>
+    let alreadyReceived := st.msgReceivedFrom msg;
+    if src ∈ alreadyReceived then
+      none
+    else
+      let msgReceivedFrom' := st.msgReceivedFrom[msg ↦ src :: alreadyReceived]
+      let st' := {st with msgReceivedFrom := msgReceivedFrom'}
+      .some (st', [])
 
 def procMsg (st : @NodeState Address Round Value) (src : Address) (msg : @Message Address Round Value) :
   (@NodeState Address Round Value) × List (Packet Address (@Message Address Round Value)) := sorry
 
-instance RBProtocol : @NetworkProtocol Address (@Message Address Round Value) (@NodeState Address Round Value) (@InternalTransition Round) :=
-  ⟨init, procInt, procMsg⟩
+instance RBProtocol (nodes : List Address) (inputValue : Address → Value) :
+  @NetworkProtocol Address (@Message Address Round Value) (@NodeState Address Round Value) (@InternalTransition Round) :=
+  ⟨λ id => init id nodes, procInt inputValue, procMsg⟩
 
-
-def RBNetworkState := @AsynchronousNetwork.World Address (Packet Address (@Message Address Round Value)) (@NodeState Address Round Value)
-instance RBAdversary : @ByzantineAdversary Address (@Message Address Round Value) (@NetworkState Address (Packet Address (@Message Address Round Value)) (@NodeState Address Round Value)) := sorry
-
--- #check AsynchronousNetwork.transition
--- #check (@defaultNetworkState _ _ _ _ RBProtocol).default
-
-instance RBAsyncNetwork
+instance RBAsyncNetwork (nodes : List Address) (inputValue : Address → Value)
   : RelationalTransitionSystem (@RBNetworkState Address Round Value) where
-  init  := λ s => s = (@defaultNetworkState _ _ _ _ RBProtocol).default
+  init  := λ s => s = @AsynchronousNetwork.init _ _ _ _ (RBProtocol nodes inputValue) nodes
   next  := λ w w' => ∃
             (s : AsynchronousNetwork.step)
-            (_ : @AsynchronousNetwork.transition _ _ _ _ _ _  RBProtocol RBAdversary s w w'), True
-            -- (t : @AsynchronousNetwork.transition Address (@Message Address Round Value) (@NodeState Address Round Value) (@InternalTransition Round) _ _  RBProtocol byz
-            --     s w w'), True
+            (_ : @AsynchronousNetwork.transition _ _ _ _ _ _  (RBProtocol nodes inputValue) RBAdversary s w w'), True
   safe := λ _ => True
   inv  := λ _ => True
 
--- #check (@invInit _ RBAsyncNetwork)
-
 namespace RBProofs
 
-theorem initInv : (@invInit (@RBNetworkState Address Round Value) RBAsyncNetwork) := by {
+theorem initInv : (@invInit (@RBNetworkState Address Round Value) (RBAsyncNetwork nodes inputValue)) := by {
   simp [invInit, RelationalTransitionSystem.init, RelationalTransitionSystem.inv]
 }
 
