LeanSts/BFT/Byzantine.lean
@@ -1,30 +1,21 @@
 import Mathlib.Tactic
 
-class ByzantineThreshold :=
+#check Finset
+
+/-- A Byzantine setting in which the Byzantine nodes are fixed ahead of time. -/
+class NonadaptiveByzantineSetting {NetAddr : Type} :=
   /-- Total number of nodes. -/
   N : ℕ
   /-- Number of permitted Byzantine faults. -/
   f : ℕ
-
-  N_gt_0 : 0 < N
-  f_lt_N : f < N
-
-instance ClassicByzantineThreshold (N : ℕ) (N_gt_0 : 0 < N) : ByzantineThreshold :=
-  ⟨N, ⌊N / 3⌋₊, N_gt_0, by simp ; omega⟩
-
-/-- A Byzantine setting in which the Byzantine nodes are fixed ahead of time. -/
-class NonadaptiveByzantineSetting {NetAddr : Type} :=
   /-- Is this node Byzantine? -/
   isByzantine : NetAddr → Bool
 
-/-- A Byzantine setting in which the Byzantine nodes potentially vary over time. -/
-class ByzantineSetting {NetAddr NetworkState : Type} :=
-  /-- Is this node Byzantine? -/
-  isByzantine : NetAddr → NetworkState → Bool
+  N_gt_0 : 0 < N
+  f_lt_N : f < N
+  -- byz_lte_f :
+  --   {n | isByzantine n = true} ≤ f
 
-/-- A non-adaptive Byzantine setting is a restricted form of the adaptive setting. -/
-instance [na : @NonadaptiveByzantineSetting NetAddr] : @ByzantineSetting NetAddr NetworkState :=
-  ⟨λ addr _ => na.isByzantine addr⟩
 
 /-- A Byzantine adversary is constrained in terms of the messages it can produce
   in a given NetworkState (which can include history information). -/
@@ -32,5 +23,5 @@ class AdversaryConstraint {Message NetworkState : Type} :=
   canProduceMessage : Message → NetworkState  → Prop
 
 class ByzantineAdversary {NetAddr Message NetworkState : Type} :=
-  setting : @ByzantineSetting NetAddr NetworkState
+  setting : @NonadaptiveByzantineSetting NetAddr
   constraint : @AdversaryConstraint Message NetworkState
